<?xml version="1.0"?>
<rdf:RDF
    xmlns:gi2mo="http://purl.org/gi2mo/ns#"
    xmlns:rdf="http://www.w3.org/1999/02/22-rdf-syntax-ns#"
    xmlns:protege="http://protege.stanford.edu/plugins/owl/protege#"
    xmlns:xsp="http://www.owl-ontologies.com/2005/08/07/xsp.owl#"
    xmlns:owl="http://www.w3.org/2002/07/owl#"
    xmlns:terms="http://purl.org/dc/terms/"
    xmlns:xsd="http://www.w3.org/2001/XMLSchema#"
    xmlns:gi2mowave="http://purl.org/gi2mo/wave/ns#"
    xmlns:swrl="http://www.w3.org/2003/11/swrl#"
    xmlns:swrlb="http://www.w3.org/2003/11/swrlb#"
    xmlns:rdfs="http://www.w3.org/2000/01/rdf-schema#"
  xml:base="http://purl.org/gi2mo/wave/ns">
  <owl:Ontology rdf:about="">
    <owl:imports rdf:resource="http://purl.org/gi2mo/ns"/>
  </owl:Ontology>
  <owl:Class rdf:ID="Competitor">
    <rdfs:label xml:lang="en">Competitor</rdfs:label>
    <rdfs:comment xml:lang="en">An object of this type indicates a competitor for an idea or IdeaContest</rdfs:comment>
  </owl:Class>
  <owl:Class rdf:ID="Market">
    <rdfs:comment xml:lang="en">An object of this type indicates the market aim by an idea or IdeaContest. It could be a place, a sector, a niche, etc</rdfs:comment>
    <rdfs:label xml:lang="en">Market</rdfs:label>
  </owl:Class>
  <owl:Class rdf:ID="Resource">
    <rdfs:comment xml:lang="en">An object of this type indicates a resource necessary for an idea or IdeaContest. 
This resource can be of different types; general, knowledge, financial, income, etc.
For a list of recommended instances of this class see the individuals list associated to this class in the ontology definition.</rdfs:comment>
    <rdfs:label xml:lang="en">Resource</rdfs:label>
  </owl:Class>
  <owl:Class rdf:ID="Target">
    <rdfs:comment xml:lang="en">An object of this type indicates the objective or target aim by an idea or IdeaContest</rdfs:comment>
    <rdfs:label xml:lang="en">Target</rdfs:label>
  </owl:Class>
  <owl:Class rdf:ID="IdeaContestType">
    <rdfs:comment xml:lang="en">An object of this type indicates the type of innovation search by the IdeaContest. 
There are 12 dimensions or types identified.
For a list of recommended instances of this class see the individuals list associated to this class in the ontology definition.</rdfs:comment>
    <rdfs:label xml:lang="en">IdeaContestType</rdfs:label>
  </owl:Class>
  <owl:Class rdf:about="http://purl.org/gi2mo/ns#User"/>
  <owl:Class rdf:ID="Outcome">
    <rdfs:comment xml:lang="en">An object of this type indicates final result or outcome for an idea or IdeaContest. 
This outcome or result can be a product, a service, a process, a strategy, an improvement, a company or spin-off or cooperation among companies, departments,etc.
For a list of recommended instances of this class see the individuals list associated to this class in the ontology definition.</rdfs:comment>
    <rdfs:label xml:lang="en">Outcome</rdfs:label>
  </owl:Class>
  <owl:Class rdf:about="http://www.w3.org/2002/07/owl#Thing"/>
  <owl:Class rdf:about="http://purl.org/gi2mo/ns#IdeaContest"/>
  <owl:Class rdf:ID="Technology">
    <rdfs:comment xml:lang="en">An object of this type indicates the technology used or proposed by an idea or IdeaContest</rdfs:comment>
    <rdfs:label xml:lang="en">Technology</rdfs:label>
  </owl:Class>
  <owl:Class rdf:about="http://purl.org/gi2mo/ns#Idea"/>
  <owl:Class rdf:ID="IdeaContestStatus">
    <rdfs:comment xml:lang="en">An instance of this class describes the status of an ideaContest and indicates the position or stage of the contest in the Idea Management life cycle (idea creation, analysis, enrichment, selection, etc) 

For a list of recommended instances of this class see the individuals list associated to this class in the ontology definition.</rdfs:comment>
  </owl:Class>
  <owl:Class rdf:ID="IdeaContestSelectionCriteria">
    <rdfs:comment xml:lang="en">An object of this type indicates the criteria used in an IdeaContest. For a list of recommended instances of this class see the individuals list associated to this class in the ontology definition.</rdfs:comment>
  </owl:Class>
  <owl:Class rdf:ID="Customer">
    <rdfs:comment xml:lang="en">An object of this type indicates the customer targeted by an idea or IdeaContest</rdfs:comment>
    <rdfs:label xml:lang="en">Customer</rdfs:label>
  </owl:Class>
  <owl:ObjectProperty rdf:ID="hasTarget">
    <rdfs:domain>
      <owl:Class>
        <owl:unionOf rdf:parseType="Collection">
          <owl:Class rdf:about="http://purl.org/gi2mo/ns#Idea"/>
          <owl:Class rdf:about="http://purl.org/gi2mo/ns#IdeaContest"/>
        </owl:unionOf>
      </owl:Class>
    </rdfs:domain>
    <rdfs:comment xml:lang="en">Property indicating an idea or other entity having an objective or target.</rdfs:comment>
    <owl:inverseOf>
      <owl:ObjectProperty rdf:ID="isTargetOf"/>
    </owl:inverseOf>
    <rdfs:label xml:lang="en">hasTarget</rdfs:label>
    <rdfs:range rdf:resource="#Target"/>
  </owl:ObjectProperty>
  <owl:ObjectProperty rdf:ID="isCustomerOf">
    <rdfs:comment xml:lang="en">Property indicating a customer is the beneficiary of an idea or other entity.</rdfs:comment>
    <rdfs:range rdf:resource="http://purl.org/gi2mo/ns#Idea"/>
    <rdfs:label xml:lang="en">isCustomerOf</rdfs:label>
    <rdfs:domain rdf:resource="#Customer"/>
  </owl:ObjectProperty>
  <owl:ObjectProperty rdf:ID="isTechnologyOf">
    <rdfs:domain rdf:resource="#Technology"/>
    <rdfs:comment xml:lang="en">Property indicating a technology is being used by an idea or other entity.</rdfs:comment>
    <rdfs:range rdf:resource="http://purl.org/gi2mo/ns#Idea"/>
  </owl:ObjectProperty>
  <owl:ObjectProperty rdf:ID="isResourceOf">
    <rdfs:range rdf:resource="http://purl.org/gi2mo/ns#Idea"/>
    <rdfs:label xml:lang="en">isResourceOf</rdfs:label>
    <rdfs:domain rdf:resource="#Resource"/>
    <rdfs:comment xml:lang="en">Property indicating a resource is being used by an idea or other entity.</rdfs:comment>
  </owl:ObjectProperty>
  <owl:ObjectProperty rdf:ID="hasCompetitor">
    <rdfs:range rdf:resource="#Competitor"/>
    <owl:inverseOf>
      <owl:ObjectProperty rdf:ID="isCompetitorOf"/>
    </owl:inverseOf>
    <rdfs:comment xml:lang="en">Property indicating an idea or other entity having a competitor in the market.</rdfs:comment>
    <rdfs:domain rdf:resource="http://purl.org/gi2mo/ns#Idea"/>
    <rdfs:label xml:lang="en">hasCompetitor</rdfs:label>
  </owl:ObjectProperty>
  <owl:ObjectProperty rdf:ID="hasResource">
    <rdfs:domain rdf:resource="http://purl.org/gi2mo/ns#Idea"/>
    <rdfs:comment xml:lang="en">Property indicating an idea or other entity having (using, depending ...) a resource.</rdfs:comment>
    <owl:inverseOf rdf:resource="#isResourceOf"/>
    <rdfs:range rdf:resource="#Resource"/>
    <rdfs:label xml:lang="en">hasResource</rdfs:label>
  </owl:ObjectProperty>
  <owl:ObjectProperty rdf:ID="isOutcomeOf">
    <rdfs:comment xml:lang="en">Property indicating an entity being the outcome or the expected outcome of an idea or other entity.</rdfs:comment>
    <rdfs:label xml:lang="en">isOutcomeOf</rdfs:label>
    <rdfs:domain rdf:resource="#Outcome"/>
    <rdfs:range rdf:resource="http://purl.org/gi2mo/ns#Idea"/>
  </owl:ObjectProperty>
  <owl:ObjectProperty rdf:ID="hasCustomer">
    <rdfs:label xml:lang="en">hasCustomer</rdfs:label>
    <rdfs:range rdf:resource="#Customer"/>
    <owl:inverseOf rdf:resource="#isCustomerOf"/>
    <rdfs:comment xml:lang="en">Property indicating an idea or other entity having a customer or possible customer.</rdfs:comment>
    <rdfs:domain rdf:resource="http://purl.org/gi2mo/ns#Idea"/>
  </owl:ObjectProperty>
  <owl:ObjectProperty rdf:ID="hasType">
    <rdfs:range rdf:resource="#IdeaContestType"/>
    <rdfs:domain rdf:resource="http://purl.org/gi2mo/ns#IdeaContest"/>
    <rdfs:label xml:lang="en">hasType</rdfs:label>
    <owl:inverseOf>
      <owl:ObjectProperty rdf:ID="isTypeOf"/>
    </owl:inverseOf>
    <rdfs:comment xml:lang="en">Property indicating an ideacontest has a type.
For a list of the possible types available see the individuals for IdeaContestType</rdfs:comment>
  </owl:ObjectProperty>
  <owl:ObjectProperty rdf:about="#isTypeOf">
    <rdfs:range rdf:resource="http://purl.org/gi2mo/ns#IdeaContest"/>
    <rdfs:comment xml:lang="en">Property indicating an ideaContestType defines the type of an IdeaContest.</rdfs:comment>
    <rdfs:domain rdf:resource="#IdeaContestType"/>
    <rdfs:label xml:lang="en">isTypeOf</rdfs:label>
  </owl:ObjectProperty>
  <owl:ObjectProperty rdf:ID="isMarketOf">
    <rdfs:comment xml:lang="en">Property indicating a market is the objective of an idea or other entity.</rdfs:comment>
    <rdfs:domain rdf:resource="#Market"/>
    <rdfs:range rdf:resource="http://purl.org/gi2mo/ns#Idea"/>
    <rdfs:label xml:lang="en">isMarketOf</rdfs:label>
  </owl:ObjectProperty>
  <owl:ObjectProperty rdf:ID="isOwnerOf">
    <rdfs:label xml:lang="en">isOwnerOf</rdfs:label>
    <rdfs:comment xml:lang="en">Property indicating a user is the owner or responsible of an idea contest or other entity.</rdfs:comment>
    <rdfs:range rdf:resource="http://purl.org/gi2mo/ns#IdeaContest"/>
    <rdfs:domain rdf:resource="http://purl.org/gi2mo/ns#User"/>
  </owl:ObjectProperty>
  <owl:ObjectProperty rdf:about="#isTargetOf">
    <rdfs:comment xml:lang="en">Property indicating an objective is being looked for by an idea or other entity.</rdfs:comment>
    <rdfs:range>
      <owl:Class>
        <owl:unionOf rdf:parseType="Collection">
          <owl:Class rdf:about="http://purl.org/gi2mo/ns#Idea"/>
          <owl:Class rdf:about="http://purl.org/gi2mo/ns#IdeaContest"/>
        </owl:unionOf>
      </owl:Class>
    </rdfs:range>
    <rdfs:domain rdf:resource="#Target"/>
    <rdfs:label xml:lang="en">isTargetOf</rdfs:label>
  </owl:ObjectProperty>
  <owl:ObjectProperty rdf:about="http://purl.org/gi2mo/ns#hasStatus">
    <rdfs:domain rdf:resource="http://purl.org/gi2mo/ns#IdeaContest"/>
    <rdfs:range rdf:resource="#IdeaContestStatus"/>
  </owl:ObjectProperty>
  <owl:ObjectProperty rdf:ID="hasSelectionCriteria">
    <rdfs:domain rdf:resource="http://purl.org/gi2mo/ns#IdeaContest"/>
    <rdfs:label xml:lang="en">hasSelectionCriteria</rdfs:label>
    <rdfs:comment xml:lang="en">Property indicating an ideaContest uses one of the IdeaContestSelectionCriteria.
For a list of the possible types of selection criteria available see the individuals for IdeaContestSelectionCriteria</rdfs:comment>
    <owl:inverseOf>
      <owl:ObjectProperty rdf:ID="isSelectionCriteriaOf"/>
    </owl:inverseOf>
    <rdfs:range rdf:resource="#IdeaContestSelectionCriteria"/>
  </owl:ObjectProperty>
  <owl:ObjectProperty rdf:ID="hasOwner">
    <rdfs:comment xml:lang="en">Property indicating an ideacontest or other entity having a user as an owner or responsible.</rdfs:comment>
    <rdfs:range rdf:resource="http://purl.org/gi2mo/ns#User"/>
    <rdfs:domain rdf:resource="http://purl.org/gi2mo/ns#IdeaContest"/>
    <rdfs:label xml:lang="en">hasOwner</rdfs:label>
    <owl:inverseOf rdf:resource="#isOwnerOf"/>
  </owl:ObjectProperty>
  <owl:ObjectProperty rdf:ID="hasTechnology">
    <rdfs:domain rdf:resource="http://purl.org/gi2mo/ns#Idea"/>
    <rdfs:comment xml:lang="en">Property indicating an idea or other entity using, employing or depending on a technology.</rdfs:comment>
    <owl:inverseOf rdf:resource="#isTechnologyOf"/>
    <rdfs:range rdf:resource="#Technology"/>
    <rdfs:label xml:lang="en">hasTechnology</rdfs:label>
  </owl:ObjectProperty>
  <owl:ObjectProperty rdf:about="#isCompetitorOf">
    <rdfs:comment xml:lang="en">Property indicating an individual or entity being competitor of an idea or other entity.</rdfs:comment>
    <rdfs:label xml:lang="en">isCompetitorOf</rdfs:label>
    <rdfs:domain rdf:resource="#Competitor"/>
    <rdfs:range rdf:resource="http://purl.org/gi2mo/ns#Idea"/>
  </owl:ObjectProperty>
  <owl:ObjectProperty rdf:ID="hasMarket">
    <owl:inverseOf rdf:resource="#isMarketOf"/>
    <rdfs:label xml:lang="en">hasMarket</rdfs:label>
    <rdfs:range rdf:resource="#Market"/>
    <rdfs:comment xml:lang="en">Property indicating an idea or other entity aiming towards a market.</rdfs:comment>
    <rdfs:domain rdf:resource="http://purl.org/gi2mo/ns#Idea"/>
  </owl:ObjectProperty>
  <owl:ObjectProperty rdf:about="#isSelectionCriteriaOf">
    <rdfs:range rdf:resource="http://purl.org/gi2mo/ns#IdeaContest"/>
    <rdfs:domain rdf:resource="#IdeaContestSelectionCriteria"/>
    <rdfs:label xml:lang="en">isSelectionCriteriaOf</rdfs:label>
    <rdfs:comment xml:lang="en">Property indicating an ideaContestSelectionCriteria defines an IdeaContest selection method.
For a list of the possible types of selection criteria available see the individuals for IdeaContestSelectionCriteria.</rdfs:comment>
  </owl:ObjectProperty>
  <owl:ObjectProperty rdf:ID="hasOutcome">
    <owl:inverseOf rdf:resource="#isOutcomeOf"/>
    <rdfs:comment xml:lang="en">Property indicating an idea or other entity having an outcome as an expectation.</rdfs:comment>
    <rdfs:range rdf:resource="#Outcome"/>
    <rdfs:label xml:lang="en">hasOutcome</rdfs:label>
    <rdfs:domain rdf:resource="http://purl.org/gi2mo/ns#Idea"/>
  </owl:ObjectProperty>
  <owl:DatatypeProperty rdf:about="http://purl.org/gi2mo/ns#content">
    <rdfs:domain>
      <owl:Class>
        <owl:unionOf rdf:parseType="Collection">
          <owl:Class rdf:about="#Competitor"/>
          <owl:Class rdf:about="#Customer"/>
          <owl:Class rdf:about="#IdeaContestSelectionCriteria"/>
          <owl:Class rdf:about="#IdeaContestStatus"/>
          <owl:Class rdf:about="#IdeaContestType"/>
          <owl:Class rdf:about="#Market"/>
          <owl:Class rdf:about="#Outcome"/>
          <owl:Class rdf:about="#Resource"/>
          <owl:Class rdf:about="#Target"/>
          <owl:Class rdf:about="#Technology"/>
        </owl:unionOf>
      </owl:Class>
    </rdfs:domain>
  </owl:DatatypeProperty>
  <owl:DatatypeProperty rdf:about="http://purl.org/gi2mo/ns#endDate">
    <rdfs:domain rdf:resource="#IdeaContestStatus"/>
  </owl:DatatypeProperty>
  <owl:DatatypeProperty rdf:about="http://purl.org/dc/terms/title">
    <rdfs:domain>
      <owl:Class>
        <owl:unionOf rdf:parseType="Collection">
          <owl:Class rdf:about="#Competitor"/>
          <owl:Class rdf:about="#Customer"/>
          <owl:Class rdf:about="#IdeaContestSelectionCriteria"/>
          <owl:Class rdf:about="#IdeaContestStatus"/>
          <owl:Class rdf:about="#IdeaContestType"/>
          <owl:Class rdf:about="#Market"/>
          <owl:Class rdf:about="#Outcome"/>
          <owl:Class rdf:about="#Resource"/>
          <owl:Class rdf:about="#Target"/>
          <owl:Class rdf:about="#Technology"/>
        </owl:unionOf>
      </owl:Class>
    </rdfs:domain>
  </owl:DatatypeProperty>
  <owl:DatatypeProperty rdf:about="http://purl.org/gi2mo/ns#startDate">
    <rdfs:domain rdf:resource="#IdeaContestStatus"/>
  </owl:DatatypeProperty>
  <owl:DatatypeProperty rdf:about="http://purl.org/dc/terms/description">
    <rdfs:domain>
      <owl:Class>
        <owl:unionOf rdf:parseType="Collection">
          <owl:Class rdf:about="#Competitor"/>
          <owl:Class rdf:about="#Customer"/>
          <owl:Class rdf:about="#IdeaContestSelectionCriteria"/>
          <owl:Class rdf:about="#IdeaContestStatus"/>
          <owl:Class rdf:about="#IdeaContestType"/>
          <owl:Class rdf:about="#Market"/>
          <owl:Class rdf:about="#Outcome"/>
          <owl:Class rdf:about="#Resource"/>
          <owl:Class rdf:about="#Target"/>
          <owl:Class rdf:about="#Technology"/>
        </owl:unionOf>
      </owl:Class>
    </rdfs:domain>
  </owl:DatatypeProperty>
  <owl:NamedIndividual rdf:about="http://172.17.200.197/investisite/rdf/schema/GI2MOWave.owl#Position_Client">
    <rdfs:comment xml:lang="en">Indicates that the type of innovation pursuit by an idea or ideacontest aims to discover requirements not cover or inarticulate, or to identify new client segments (niche).</rdfs:comment>
    <rdfs:label xml:lang="en">Position_Client</rdfs:label>
    <rdf:type rdf:resource="#Outcome"/>
    <rdf:type rdf:resource="#IdeaContestType"/>
  </owl:NamedIndividual>
  <owl:NamedIndividual rdf:about="http://172.17.200.197/investisite/rdf/schema/GI2MOWave.owl#Strategy">
    <rdfs:label xml:lang="en">Strategy</rdfs:label>
    <rdf:type rdf:resource="#Outcome"/>
    <rdfs:comment xml:lang="en">Indicates that the expected outcome for an idea or ideacontest is to become a strategy or that an idea has already become a strategy. The status of an idea or ideacontest need to be known in advance in order to resolve whether the idea has materialized or not.</rdfs:comment>
  </owl:NamedIndividual>
  <owl:NamedIndividual rdf:about="http://172.17.200.197/investisite/rdf/schema/GI2MOWave.owl#Joint">
    <rdf:type rdf:resource="#Outcome"/>
    <rdfs:comment xml:lang="en">Indicates that the expected outcome for an idea or ideacontest is to become a joint venture, cooperation or similar, or that an idea has already become a joint venture, cooperation or similar. The status of an idea or ideacontest need to be known in advance in order to resolve whether the idea has materialized or not.</rdfs:comment>
    <rdfs:label xml:lang="en">Joint</rdfs:label>
  </owl:NamedIndividual>
  <owl:AnnotationProperty rdf:about="http://www.w3.org/2000/01/rdf-schema#comment"/>
  <owl:NamedIndividual rdf:about="http://172.17.200.197/investisite/rdf/schema/GI2MOWave.owl#Product_Solution">
    <rdfs:label xml:lang="en">Product_Solution</rdfs:label>
    <rdfs:comment xml:lang="en">Indicates that the type of innovation pursuit by an idea or ideacontest is to become a solution that integrates combinations of products and services that solve customer needs from end to end.</rdfs:comment>
    <rdf:type rdf:resource="#Outcome"/>
    <rdf:type rdf:resource="#IdeaContestType"/>
  </owl:NamedIndividual>
  <owl:NamedIndividual rdf:about="http://172.17.200.197/investisite/rdf/schema/GI2MOWave.owl#Service">
    <rdfs:label xml:lang="en">Service</rdfs:label>
    <rdf:type rdf:resource="#Outcome"/>
    <rdfs:comment xml:lang="en">Indicates that the expected outcome for an idea or ideacontest is to become a service or that an idea has already become a service. The status of an idea or ideacontest need to be known in advance in order to resolve whether the idea has materialized or not.</rdfs:comment>
  </owl:NamedIndividual>
  <owl:NamedIndividual rdf:about="http://172.17.200.197/investisite/rdf/schema/GI2MOWave.owl#Paradigma_Capture_Value">
    <rdfs:label xml:lang="en">Paradigma_Capture_Value</rdfs:label>
    <rdf:type rdf:resource="#Outcome"/>
    <rdf:type rdf:resource="#IdeaContestType"/>
    <rdfs:comment xml:lang="en">Indicates that the type of innovation pursuit by an idea or ideacontest aims to discover new income sources for the company or redefine the way the company is paid.</rdfs:comment>
  </owl:NamedIndividual>
  <owl:NamedIndividual rdf:about="http://172.17.200.197/investisite/rdf/schema/GI2MOWave.owl#IdeaAnalisysState">
    <rdf:type rdf:resource="#IdeaContestStatus"/>
    <rdfs:label xml:lang="en">IdeaAnalisysState</rdfs:label>
    <rdfs:comment xml:lang="en">At this stage ideas are analysed. Similar ideas are merged, an idea can be split into several ideas, relation with other ideas (actual or previous) is searched for and other similar tasks are performed at this stage.</rdfs:comment>
  </owl:NamedIndividual>
  <owl:NamedIndividual rdf:about="http://172.17.200.197/investisite/rdf/schema/GI2MOWave.owl#Process_Organization">
    <rdfs:label xml:lang="en">Process_Organization
</rdfs:label>
    <rdf:type rdf:resource="#Outcome"/>
    <rdf:type rdf:resource="#IdeaContestType"/>
    <rdfs:comment xml:lang="en">Indicates that the type of innovation pursuit by an idea or ideacontest aims to redefine activity targets and scope for the company, functions, responsibilities and stimulus for the company units and individuals.</rdfs:comment>
  </owl:NamedIndividual>
  <owl:NamedIndividual rdf:about="http://172.17.200.197/investisite/rdf/schema/GI2MOWave.owl#Paradigma_Network">
    <rdfs:comment xml:lang="en">Indicates that the type of innovation pursuit by an idea or ideacontest aims to take advantage of the network provided by the company to its customers to add further value.</rdfs:comment>
    <rdfs:label xml:lang="en">Paradigma_Network</rdfs:label>
    <rdf:type rdf:resource="#Outcome"/>
    <rdf:type rdf:resource="#IdeaContestType"/>
  </owl:NamedIndividual>
  <owl:NamedIndividual rdf:about="http://172.17.200.197/investisite/rdf/schema/GI2MOWave.owl#Product_Platform">
    <rdf:type rdf:resource="#Outcome"/>
    <rdf:type rdf:resource="#IdeaContestType"/>
    <rdfs:comment xml:lang="en">Indicates that the type of innovation pursuit by an idea or ideacontest is  to become a group of components or technologies that allow the efficient development of lines or products.</rdfs:comment>
    <rdfs:label xml:lang="en">Product_Platform</rdfs:label>
  </owl:NamedIndividual>
  <owl:NamedIndividual rdf:about="http://172.17.200.197/investisite/rdf/schema/GI2MOWave.owl#IdeaEnrichmentState">
    <rdf:type rdf:resource="#IdeaContestStatus"/>
    <rdfs:comment xml:lang="en">At this stage ideas are published so other collaborators make their contributions; new content can be added, links to other ideas or knowledge can be attached, comments can be placed or possible partners identified.</rdfs:comment>
    <rdfs:label xml:lang="en">IdeaEnrichmentState</rdfs:label>
  </owl:NamedIndividual>
  <owl:NamedIndividual rdf:about="http://172.17.200.197/investisite/rdf/schema/GI2MOWave.owl#IdeaCreationState">
    <rdf:type rdf:resource="#IdeaContestStatus"/>
    <rdfs:comment xml:lang="en">This is the first stage in the innovation process. At this stage ideas are gathered in the platform.</rdfs:comment>
    <rdfs:label xml:lang="en">IdeaCreationState</rdfs:label>
  </owl:NamedIndividual>
  <owl:NamedIndividual rdf:about="http://172.17.200.197/investisite/rdf/schema/GI2MOWave.owl#Position_Presence">
    <rdfs:comment xml:lang="en">Indicates that the type of innovation pursuit by an idea or ideacontest aims to create new distribution channels or redefine the selling points (where customers buy or use products and services)</rdfs:comment>
    <rdf:type rdf:resource="#Outcome"/>
    <rdf:type rdf:resource="#IdeaContestType"/>
    <rdfs:label xml:lang="en">Position_Presence</rdfs:label>
  </owl:NamedIndividual>
  <owl:AnnotationProperty rdf:about="http://www.w3.org/2000/01/rdf-schema#label"/>
  <owl:NamedIndividual rdf:about="http://172.17.200.197/investisite/rdf/schema/GI2MOWave.owl#Patent">
    <rdfs:comment xml:lang="en">Indicates that the expected outcome for an idea or ideacontest is to become a patent or that an idea has already become a patent. The status of an idea or ideacontest need to be known in advance in order to resolve whether the idea has materialized or not.</rdfs:comment>
    <rdf:type rdf:resource="#Outcome"/>
  </owl:NamedIndividual>
  <owl:NamedIndividual rdf:about="http://172.17.200.197/investisite/rdf/schema/GI2MOWave.owl#CriteriaMatrix">
    <rdfs:comment xml:lang="en">It is a selection method where the owner of the process sets the values to be assigned to the different options.</rdfs:comment>
    <rdf:type rdf:resource="#IdeaContestSelectionCriteria"/>
    <rdfs:label xml:lang="en">CriteriaMatrix</rdfs:label>
  </owl:NamedIndividual>
  <owl:NamedIndividual rdf:about="http://172.17.200.197/investisite/rdf/schema/GI2MOWave.owl#Position_Experience">
    <rdfs:comment xml:lang="en">Indicates that the type of innovation pursuit by an idea or ideacontest aims to redesign customer relations in every stage of the process.</rdfs:comment>
    <rdf:type rdf:resource="#Outcome"/>
    <rdf:type rdf:resource="#IdeaContestType"/>
    <rdfs:label xml:lang="en">Position_Experience</rdfs:label>
  </owl:NamedIndividual>
  <owl:NamedIndividual rdf:about="http://172.17.200.197/investisite/rdf/schema/GI2MOWave.owl#IdeaSelectionState">
    <rdf:type rdf:resource="#IdeaContestStatus"/>
    <rdfs:comment xml:lang="en">At this stage ideas are selected according the selection criteria established during the idea contest.</rdfs:comment>
    <rdfs:label xml:lang="en">IdeaSelectionState</rdfs:label>
  </owl:NamedIndividual>
  <owl:NamedIndividual rdf:about="http://172.17.200.197/investisite/rdf/schema/GI2MOWave.owl#Product">
    <rdfs:label xml:lang="en">Product</rdfs:label>
    <rdfs:comment xml:lang="en">Indicates that the expected outcome for an idea or ideacontest is to become a product or that an idea has already become a product. The status of an idea or ideacontest need to be known in advance in order to resolve whether the idea has materialized or not.</rdfs:comment>
    <rdf:type rdf:resource="#Outcome"/>
  </owl:NamedIndividual>
  <owl:NamedIndividual rdf:about="http://172.17.200.197/investisite/rdf/schema/GI2MOWave.owl#PonderatedSelection">
    <rdfs:comment xml:lang="en">PonderatedSelection is a selection criteria method that takes into account quality aspects. It is used when quantity aspects cannot be measured. It reduces subjectivity and looks for group agreements.</rdfs:comment>
    <rdf:type rdf:resource="#IdeaContestSelectionCriteria"/>
    <rdfs:label xml:lang="en">PonderatedSelection</rdfs:label>
  </owl:NamedIndividual>
  <owl:NamedIndividual rdf:about="http://172.17.200.197/investisite/rdf/schema/GI2MOWave.owl#Process_Process">
    <rdfs:label xml:lang="en">Process_Process</rdfs:label>
    <rdf:type rdf:resource="#Outcome"/>
    <rdf:type rdf:resource="#IdeaContestType"/>
    <rdfs:comment xml:lang="en">Indicates that the type of innovation pursuit by an idea or ideacontest aims to design and group activities to achieve more efficiency, higher quality and faster responses in processes.</rdfs:comment>
  </owl:NamedIndividual>
  <owl:NamedIndividual rdf:about="http://172.17.200.197/investisite/rdf/schema/GI2MOWave.owl#Process">
    <rdfs:comment xml:lang="en">Indicates that the expected outcome for an idea or ideacontest is to become a process or that an idea has already become a process. The status of an idea or ideacontest need to be known in advance in order to resolve whether the idea has materialized or not.</rdfs:comment>
    <rdf:type rdf:resource="#Outcome"/>
  </owl:NamedIndividual>
  <owl:NamedIndividual rdf:about="http://172.17.200.197/investisite/rdf/schema/GI2MOWave.owl#NormalPonderation">
    <rdfs:label xml:lang="en">NormalPonderation</rdfs:label>
    <rdf:type rdf:resource="#IdeaContestSelectionCriteria"/>
    <rdfs:comment xml:lang="en">Idea selection criteria that give ideas values ranging from 0 to 10</rdfs:comment>
  </owl:NamedIndividual>
  <owl:NamedIndividual rdf:about="http://172.17.200.197/investisite/rdf/schema/GI2MOWave.owl#Product_Offer">
    <rdfs:label xml:lang="en">Product_Offer</rdfs:label>
    <rdf:type rdf:resource="#Outcome"/>
    <rdf:type rdf:resource="#IdeaContestType"/>
    <rdfs:comment xml:lang="en">Indicates that the type of innovation pursuit by an idea or ideacontest is to become a new product or service that adds value to customer needs.</rdfs:comment>
  </owl:NamedIndividual>
  <owl:NamedIndividual rdf:about="http://172.17.200.197/investisite/rdf/schema/GI2MOWave.owl#Company">
    <rdf:type rdf:resource="#Outcome"/>
    <rdfs:comment xml:lang="en">Indicates that the expected outcome for an idea or ideacontest is to become a company, spin-off or similar or that an idea has already become a company, spin-off or similar. The status of an idea or ideacontest need to be known in advance in order to resolve whether the idea has materialized or not.</rdfs:comment>
    <rdfs:label xml:lang="en">Company</rdfs:label>
  </owl:NamedIndividual>
  <owl:NamedIndividual rdf:about="http://172.17.200.197/investisite/rdf/schema/GI2MOWave.owl#IdeaDevelopmentState">
    <rdfs:comment xml:lang="en">At this stage the idea is developed to obtain an outcome. The outcome of an idea can be of different nature (see outcome).</rdfs:comment>
    <rdf:type rdf:resource="#IdeaContestStatus"/>
    <rdfs:label xml:lang="en">IdeaDevelopmentState</rdfs:label>
  </owl:NamedIndividual>
  <owl:NamedIndividual rdf:about="http://172.17.200.197/investisite/rdf/schema/GI2MOWave.owl#Position_Brand">
    <rdfs:comment xml:lang="en">Indicates that the type of innovation pursuit by an idea or ideacontest aims to expand the brand or enter new domains.</rdfs:comment>
    <rdf:type rdf:resource="#Outcome"/>
    <rdf:type rdf:resource="#IdeaContestType"/>
    <rdfs:label xml:lang="en">Position_Brand</rdfs:label>
  </owl:NamedIndividual>
  <owl:NamedIndividual rdf:about="http://172.17.200.197/investisite/rdf/schema/GI2MOWave.owl#Process_Supply_Change">
    <rdfs:comment xml:lang="en">Indicates that the type of innovation pursuit by an idea or ideacontest aims to redesign aspects of the supply chain from provider to customer looking for better management and collaboration.</rdfs:comment>
    <rdfs:label xml:lang="en">Process_Supply_Change</rdfs:label>
    <rdf:type rdf:resource="#Outcome"/>
    <rdf:type rdf:resource="#IdeaContestType"/>
  </owl:NamedIndividual>
</rdf:RDF>

<!-- Created with Protege (with OWL Plugin 3.4, Build 533)  http://protege.stanford.edu -->
